wip

cava2/TLUL.v
@@ -133,7 +133,7 @@ Section Var.
   Definition sha_digest := Vec sha_word 8.
 
   Definition tlul_adapter_state :=
-    (BitVec TL_AIW ** BitVec TL_SZW ** BitVec 3 ** Bit ** Bit ** Bit ** Bit)%circuit_type.
+    (BitVec TL_AIW ** BitVec TL_SZW ** BitVec 3 ** BitVec 32 ** Bit ** Bit ** Bit ** Bit)%circuit_type.
 
   (* Convert TLUL packets to a simple read/write register interface *)
   (* This is similar to OpenTitan's tlul_adapter_reg, but for simplicity we
@@ -155,7 +155,9 @@ Section Var.
       , a_user
       ; d_ready) := incoming_tlp in
 
-    let/delay '(reqid, reqsz, rspop, error, outstanding, we_o; re_o) :=
+    let/delay '(reqid, reqsz, rspop, reqaddress, error, outstanding,
+                (* output only signals: *)
+                we_o; re_o) :=
 
       let a_ack := a_valid && !outstanding in
       let d_ack := outstanding && d_ready in
@@ -168,24 +170,25 @@ Section Var.
       let err_internal := `Zero` in
       let error_i := `Zero` in
 
-      let '(reqid, reqsz, rspop, error; outstanding) :=
-        if a_ack then
-          ( a_source
-          , a_size
-          , if rd_req then `K AccessAckData` else `K AccessAck`
-          , error_i || err_internal
-          , `One`
-          )
-        else
-          (reqid, reqsz, rspop, error, if d_ack then `Zero` else outstanding)
+      let '(reqid, reqsz, rspop, reqaddress, error; outstanding) :=
+          if a_ack then
+            ( a_source
+              , a_size
+              , if rd_req then `K AccessAckData` else `K AccessAck`
+              , a_address
+              , error_i || err_internal
+              , `One`
+            )
+          else
+            (reqid, reqsz, rspop, reqaddress, error, if d_ack then `Zero` else outstanding)
       in
 
       let we_o := wr_req && !err_internal in
       let re_o := rd_req && !err_internal in
 
-      (reqid, reqsz, rspop, error, outstanding, we_o, re_o)
-      initially (0,(0,(0,(false,(false,(false,false))))))
-        : denote_type (BitVec _ ** BitVec _ ** BitVec _ ** Bit ** Bit ** Bit ** Bit)
+      (reqid, reqsz, rspop, reqaddress, error, outstanding, we_o, re_o)
+      initially default
+        : denote_type (BitVec _ ** BitVec _ ** BitVec _ ** BitVec _ ** Bit ** Bit ** Bit ** Bit)
     in
 
     let wdata_o := a_data in
@@ -197,7 +200,7 @@ Section Var.
       , reqsz
       , reqid
       , `K 0`
-      , `index` registers (`bvslice 2 30` a_address)
+      , `index` registers (`bvslice 2 30` reqaddress)
       , `K 0`
       , error
       , !outstanding
@@ -210,7 +213,7 @@ End Var.
 
 Ltac destruct_tlul_adapter_reg_state reg_count :=
   destruct_state (tlul_adapter_reg (var:=denote_type) (reg_count:=reg_count))
-                 ipattern:((?reqid, (?reqsz, (?rspop, (?error, (?outstanding, (?we_o, ?re_o))))))).
+                 ipattern:((?reqid, (?reqsz, (?rspop, (?reqaddress, (?error, (?outstanding, (?we_o, ?re_o)))))))).
 
 Section StateGetters.
   Definition var : tvar := denote_type.
@@ -222,6 +225,9 @@ Section StateGetters.
     : N := ltac:(destruct_tlul_adapter_reg_state reg_count; apply reqsz).
   Definition tlul_adapter_reg_state_rspop (s : denote_type (state_of (tlul_adapter_reg (reg_count:=reg_count))))
     : N := ltac:(destruct_tlul_adapter_reg_state reg_count; apply rspop).
+  Definition tlul_adapter_reg_state_reqaddress (s : denote_type (state_of (tlul_adapter_reg (reg_count:=reg_count))))
+    : N := ltac:(destruct_tlul_adapter_reg_state reg_count; apply reqaddress).
+
   Definition tlul_adapter_reg_state_error (s : denote_type (state_of (tlul_adapter_reg (reg_count:=reg_count))))
     : bool := ltac:(destruct_tlul_adapter_reg_state reg_count; apply error).
   Definition tlul_adapter_reg_state_outstanding (s : denote_type (state_of (tlul_adapter_reg (reg_count:=reg_count))))
@@ -234,9 +240,9 @@ End StateGetters.
 
 Ltac tlul_adapter_reg_state_simpl :=
   cbn [tlul_adapter_reg_state_reqid tlul_adapter_reg_state_reqsz
-       tlul_adapter_reg_state_rspop tlul_adapter_reg_state_error
-       tlul_adapter_reg_state_outstanding tlul_adapter_reg_state_we_o
-       tlul_adapter_reg_state_re_o] in *.
+       tlul_adapter_reg_state_rspop tlul_adapter_reg_state_reqaddress
+       tlul_adapter_reg_state_error tlul_adapter_reg_state_outstanding
+       tlul_adapter_reg_state_we_o tlul_adapter_reg_state_re_o] in *.
 
 Definition tl_h2d := denote_type tl_h2d_t.
 Definition tl_h2d_default := default (t := tl_h2d_t).
@@ -344,41 +350,45 @@ Ltac tlsimpl :=
        set_d_sink set_d_data set_d_user set_d_error set_a_ready
        d_valid d_opcode d_param d_size d_source d_sink d_data d_user d_error a_ready] in *.
 
-Section TLULSpec.
+Section TLSpec.
   Local Open Scope N_scope.
 
   Context {reg_count : nat}.
 
-  Variant TLULState :=
-  | OutstandingGet (reqid : N) (reqsz : N)
-  | OutstandingPutFullData (reqid : N).
+  Variant repr_state :=
+  | Idle
+  | OutstandingAccessAckData (h2d : tl_h2d) (regs : list N)
+  | OutstandingAccessAck (h2d : tl_h2d).
 
-
-  Fixpoint outstanding_h2d (inputs : list tl_h2d) :=
-    match inputs with
-    | [] => None
-    | h :: tl =>
-      match outstanding_h2d tl with
-      | None => if a_valid h then Some h else None
-      | Some h' => if d_ready h then None else Some h'
-      end
+  Definition update_repr_state (input : denote_type (input_of (tlul_adapter_reg (reg_count:=reg_count)))) repr :=
+    let '(h2d, (regs, tt)) := input in
+    match repr with
+    | Idle =>
+      if a_valid h2d then
+        if a_opcode h2d =? Get then
+          OutstandingAccessAckData h2d regs
+        else if a_opcode h2d =? PutFullData then
+               OutstandingAccessAck h2d
+             else (* unreachable *) repr
+      else
+        repr
+    | _ =>
+      if d_ready h2d then Idle
+      else match repr with
+           | OutstandingAccessAckData h2d _ => OutstandingAccessAckData h2d regs
+           | _ => repr
+           end
     end.
 
-  Definition tlul_repr := list tl_h2d.
+  Instance tl_specification
+    : specification_for (tlul_adapter_reg (reg_count:=reg_count)) repr_state :=
+    {| reset_repr := Idle;
 
-  Instance tlul_specification
-    : specification_for (tlul_adapter_reg (reg_count:=reg_count)) tlul_repr :=
-    {| reset_repr := [];
-
-       update_repr :=
-         fun (input : denote_type (input_of (tlul_adapter_reg (reg_count:=reg_count))))
-           (repr : tlul_repr) =>
-           let '(h2d, (_regs, tt)) := input in
-           h2d :: repr;
+       update_repr := update_repr_state;
 
        precondition :=
          fun (input : denote_type (input_of tlul_adapter_reg))
-           (repr : tlul_repr) =>
+           (repr : repr_state) =>
            let '(h2d, (regs, tt)) := input in
            reg_count = length regs
            /\ (a_valid h2d = true
@@ -386,14 +396,14 @@ Section TLULSpec.
 
        postcondition :=
          fun (input : denote_type (input_of (tlul_adapter_reg (reg_count:=reg_count))))
-           (repr : tlul_repr)
+           (repr : repr_state)
            (output : denote_type (output_of (tlul_adapter_reg (reg_count:=reg_count)))) =>
-           exists h2d regs d2h io_re io_we io_address io_data io_mask,
+           exists h2d regs repr' d2h io_re io_we io_address io_data io_mask,
                input = (h2d, (regs, tt))
                /\ output = (d2h, (io_re, (io_we, (io_address, (io_data, io_mask)))))
-
-               /\ match outstanding_h2d (h2d :: repr) with
-                 | None =>
+               /\ repr' = update_repr_state input repr
+               /\ match repr' with
+                 | Idle =>
                    d_valid    d2h = false
                    /\ d_param  d2h = 0
                    /\ d_sink   d2h = 0
@@ -403,39 +413,39 @@ Section TLULSpec.
                    /\ io_re = false
                    /\ io_we = false
 
-                 | Some h2d' =>
-                   if a_opcode h2d' =? Get then
+                 | OutstandingAccessAckData h2d regs =>
                      d_valid    d2h = true
                      /\ d_opcode d2h = AccessAckData
                      /\ d_param  d2h = 0
-                     /\ d_size   d2h = a_size h2d'
-                     /\ d_source d2h = a_source h2d'
+                     /\ d_size   d2h = (a_size h2d)
+                     /\ d_source d2h = (a_source h2d)
                      /\ d_sink   d2h = 0
-                     /\ d_data   d2h = List.nth (N.to_nat (((a_address h2d / 4) mod (2 ^ 30)))) regs 0%N
+                     /\ d_data   d2h = (List.nth (N.to_nat ((((a_address h2d) / 4) mod (2 ^ 30)))) regs 0%N)
                      /\ d_user   d2h = 0
                      /\ d_error  d2h = false
                      /\ a_ready  d2h = false
-                     /\ match outstanding_h2d repr with
-                       | None => if a_valid h2d then
+                     /\ match repr with
+                       | Idle => if a_valid h2d then
                                   io_re = true
                                   /\ io_address = a_address h2d
                                 else io_re = false
                        | _ => io_re = false
                        end
                      /\ io_we = false
-                   else if a_opcode h2d' =? PutFullData then
+
+                 | OutstandingAccessAck h2d  =>
                           d_valid    d2h = true
                           /\ d_opcode d2h = AccessAck
                           /\ d_param  d2h = 0
                           (* /\ d_size   d2h =  *)
-                          /\ d_source d2h = a_source h2d'
+                          /\ d_source d2h = (a_source h2d)
                           /\ d_sink   d2h = 0
                           /\ d_user   d2h = 0
                           /\ d_error  d2h = false
                           /\ a_ready  d2h = false
                           /\ io_re = false
-                          /\ match outstanding_h2d repr with
-                            | None => if a_valid h2d then
+                          /\ match repr with
+                            | Idle => if a_valid h2d then
                                        io_we = true
                                        /\ io_address = a_address h2d
                                        /\ io_data = a_data h2d
@@ -443,30 +453,28 @@ Section TLULSpec.
                                      else io_we = false
                             | _ => io_we = false
                             end
-                        else True
-                 end
+                 end;
     |}.
 
-  Global Instance tlul_invariant : invariant_for (tlul_adapter_reg (reg_count:=reg_count)) tlul_repr :=
+  Global Instance tlul_invariant : invariant_for (tlul_adapter_reg (reg_count:=reg_count)) repr_state :=
     fun (state : denote_type (state_of tlul_adapter_reg)) repr =>
-      Forall (fun h2d => (a_valid h2d = true
-                       -> (a_opcode h2d = Get \/ a_opcode h2d = PutFullData)))
-             repr
-      /\ tlul_adapter_reg_state_error state = false
-      /\ match outstanding_h2d repr with
-        | None =>
+      tlul_adapter_reg_state_error state = false
+      /\ match repr with
+        | Idle =>
           tlul_adapter_reg_state_outstanding (reg_count:=reg_count) state = false
-        | Some h2d =>
-          if a_opcode h2d =? Get then
-            tlul_adapter_reg_state_outstanding state = true
-            /\ tlul_adapter_reg_state_reqid state = a_source h2d
-            /\ tlul_adapter_reg_state_reqsz state = a_size h2d
-            /\ tlul_adapter_reg_state_rspop state = AccessAckData
-          else if a_opcode h2d =? PutFullData then
-                 tlul_adapter_reg_state_outstanding state = true
-                 /\ tlul_adapter_reg_state_reqid state = a_source h2d
-                 /\ tlul_adapter_reg_state_rspop state = AccessAck
-               else False
+        | OutstandingAccessAckData h2d regs =>
+          tlul_adapter_reg_state_outstanding state = true
+          /\ tlul_adapter_reg_state_reqid state = (a_source h2d)
+          /\ tlul_adapter_reg_state_reqsz state = (a_size h2d)
+          /\ tlul_adapter_reg_state_rspop state = AccessAckData
+          /\ tlul_adapter_reg_state_reqaddress state = (a_address h2d)
+          /\ reg_count = length regs
+          /\ a_opcode h2d = Get
+        | OutstandingAccessAck h2d =>
+          tlul_adapter_reg_state_outstanding state = true
+          /\ tlul_adapter_reg_state_reqid state = (a_source h2d)
+          /\ tlul_adapter_reg_state_rspop state = AccessAck
+          /\ a_opcode h2d = PutFullData
         end.
 
     Lemma tlul_adapter_reg_invariant_at_reset : invariant_at_reset tlul_adapter_reg.
@@ -479,72 +487,26 @@ Section TLULSpec.
 
     Lemma tlul_adapter_reg_invariant_preserved : invariant_preserved tlul_adapter_reg.
     Proof.
-      intros (h2d, (regs, t)) state repr. destruct t.
+      intros (h2d & regs & t) state repr. destruct t.
       cbn in state. destruct_tlul_adapter_reg_state reg_count.
       destruct_tl_h2d.
       intros; subst.
       simplify_invariant (tlul_adapter_reg (reg_count:=reg_count)).
       simplify_spec (tlul_adapter_reg (reg_count:=reg_count)).
-      cbv [tlul_adapter_reg].
-      stepsimpl.
+      cbv [tlul_adapter_reg]. stepsimpl.
       tlul_adapter_reg_state_simpl. tlsimpl.
       logical_simplify.
-      match goal with
-      | h : reg_count = _ |- _ => clear h
-      end.
       repeat (destruct_pair_let; cbn [fst snd]).
       tlul_adapter_reg_state_simpl.
+      subst.
       ssplit.
-      - apply Forall_cons; assumption.
-      - destruct (a_valid0 && negb outstanding)%bool; subst; reflexivity.
-      - remember (outstanding_h2d
-                    ((a_valid0,
-                      (a_opcode0,
-                       (a_param0, (a_size0, (a_source0, (a_address0, (a_mask0, (a_data0, (a_user0, d_ready0))))))))) :: repr)) as outs eqn:Eouts.
-        destruct outs; subst.
-        + simpl in Eouts.
-          remember (outstanding_h2d repr) as outs' eqn:Eouts'.
-          destruct outs'; subst.
-          * destruct d_ready0; subst.
-            -- discriminate Eouts.
-            -- inversion Eouts; subst; clear Eouts.
-               destruct (a_opcode t0 =? Get).
-               ++ logical_simplify. subst. boolsimpl.
-                  ssplit; reflexivity.
-               ++ destruct (a_opcode t0 =? PutFullData).
-                  ** logical_simplify. subst. boolsimpl.
-                     ssplit; reflexivity.
-                  ** auto.
-          * destruct a_valid0.
-            -- inversion Eouts; subst; clear Eouts.
-               cbn.
-               destruct (a_opcode0 =? Get) eqn:Hget.
-               ++ ssplit; reflexivity.
-               ++ destruct (a_opcode0 =? PutFullData) eqn:Hput.
-                  ** ssplit; reflexivity.
-                  ** apply N.eqb_neq in Hget, Hput.
-                     destruct H1.
-                     --- reflexivity.
-                     --- apply Hget. assumption.
-                     --- apply Hput. assumption.
-            -- discriminate Eouts.
-        + simpl in Eouts.
-          remember (outstanding_h2d repr) as outs' eqn:Eouts'.
-          destruct outs'; subst.
-          -- destruct (a_opcode t =? Get) eqn:Hget.
-             ++ logical_simplify; subst. boolsimpl.
-                destruct d_ready0.
-                ** reflexivity.
-                ** discriminate Eouts.
-             ++ destruct (a_opcode t =? PutFullData) eqn:Hput.
-                ** logical_simplify; subst. boolsimpl.
-                   destruct d_ready0.
-                   --- reflexivity.
-                   --- discriminate Eouts.
-                ** exfalso. assumption.
-          -- destruct a_valid0.
-             +++ discriminate Eouts.
-             +++ boolsimpl. reflexivity.
+      - destruct (a_valid0 && negb outstanding)%bool; reflexivity.
+      - unfold update_repr_state.
+        destruct repr; [destruct a_valid0 | destruct d_ready0 ..];
+          tlsimpl; boolsimpl.
+        2-6: logical_simplify; subst outstanding; boolsimpl; ssplit; try reflexivity; assumption.
+        destruct H1; [reflexivity|..]; subst outstanding a_opcode0; cbn; [|auto].
+        ssplit; try reflexivity; assumption.
     Qed.
 
     Lemma tlul_adapter_reg_output_correct : output_correct tlul_adapter_reg.
@@ -558,143 +520,29 @@ Section TLULSpec.
       simplify_spec (tlul_adapter_reg (reg_count:=reg_count)).
       cbv [tlul_adapter_reg]. stepsimpl. logical_simplify.
       tlul_adapter_reg_state_simpl. tlsimpl.
-      rewrite List.resize_noop by assumption.
-      match goal with
-      | h : reg_count = _ |- _ => clear h
-      end.
+      (* match goal with *)
+      (* | h : reg_count = _ |- _ => clear h *)
+      (* end. *)
       subst.
       repeat (destruct_pair_let; cbn [fst snd]).
-      remember (outstanding_h2d
-                  ((a_valid0,
-                    (a_opcode0,
-                     (a_param0, (a_size0, (a_source0, (a_address0, (a_mask0, (a_data0, (a_user0, d_ready0))))))))) :: repr)) as outs eqn:Eouts.
-      destruct outs; subst.
-      - simpl in Eouts.
-        remember (outstanding_h2d repr) as outs' eqn:Eouts'.
-        destruct outs'; subst;
-          destruct d_ready0; try discriminate Eouts; inversion Eouts; subst; clear Eouts.
-        + destruct (a_opcode t0 =? Get) eqn:Hget; logical_simplify; subst; boolsimpl.
-          * do 8 eexists. split. 1: reflexivity.
-            cbn -[N.ones]. split. 1: reflexivity.
-            subst. rewrite <- Eouts'. rewrite Hget. tlsimpl.
-            ssplit; try reflexivity.
-            rewrite N.land_ones.
-            replace 4 with (2 ^ 2) by reflexivity.
-            rewrite <- ! N.shiftr_div_pow2.
-            reflexivity.
-          * destruct (a_opcode t0 =? PutFullData) eqn:Hput; logical_simplify; subst; boolsimpl.
-            -- do 8 eexists. split. 1: reflexivity.
-               cbn -[N.ones]. split. 1: reflexivity.
-               subst. rewrite <- Eouts'. rewrite Hget, Hput. tlsimpl.
-               ssplit; reflexivity.
-            -- exfalso. assumption.
-        + destruct a_valid0; try discriminate H1.
-          inversion H1; subst. clear H1.
-          do 8 eexists. split. 1: reflexivity.
-          cbn -[N.ones]. split. 1: reflexivity.
-          subst. rewrite <- Eouts'. tlsimpl.
-          destruct H3.
-          * reflexivity.
-          * subst. boolsimpl. cbn -[N.ones].
-            ssplit; try reflexivity.
-            rewrite N.land_ones.
-            replace 4 with (2 ^ 2) by reflexivity.
-            rewrite <- ! N.shiftr_div_pow2.
-            reflexivity.
-          * subst. boolsimpl. cbn. ssplit; reflexivity.
-        + destruct a_valid0; try discriminate H1.
-          inversion H1; subst. clear H1.
-          do 8 eexists. split. 1: reflexivity.
-          cbn -[N.ones]. split. 1: reflexivity.
-          subst. rewrite <- Eouts'. tlsimpl.
-          destruct H3.
-          * reflexivity.
-          * subst. boolsimpl. cbn -[N.ones].
-            ssplit; try reflexivity.
-            rewrite N.land_ones.
-            replace 4 with (2 ^ 2) by reflexivity.
-            rewrite <- ! N.shiftr_div_pow2.
-            reflexivity.
-          * subst. boolsimpl. cbn. ssplit; reflexivity.
-      - simpl in Eouts.
-        remember (outstanding_h2d repr) as outs' eqn:Eouts'.
-        destruct outs'; subst;
-          destruct d_ready0; try discriminate Eouts; inversion Eouts; subst; clear Eouts.
-        + destruct (a_opcode t =? Get) eqn:Hget; logical_simplify; subst; boolsimpl.
-          * do 8 eexists. split. 1: reflexivity.
-            cbn -[N.ones]. split. 1: reflexivity.
-            subst. rewrite <- Eouts'. tlsimpl.
-            ssplit; reflexivity.
-          * destruct (a_opcode t =? PutFullData) eqn:Hput; logical_simplify; subst; boolsimpl.
-            -- do 8 eexists. split. 1: reflexivity.
-               cbn -[N.ones]. split. 1: reflexivity.
-               subst. rewrite <- Eouts'. tlsimpl.
-               ssplit; reflexivity.
-            -- exfalso. assumption.
-        + destruct a_valid0; try discriminate H1.
-          clear H1.
-          do 8 eexists. split. 1: reflexivity.
-          cbn -[N.ones]. split. 1: reflexivity.
-          subst. rewrite <- Eouts'. tlsimpl.
-          ssplit; reflexivity.
-        + destruct a_valid0; try discriminate H1.
-          clear H1.
-          do 8 eexists. split. 1: reflexivity.
-          cbn -[N.ones]. split. 1: reflexivity.
-          subst. rewrite <- Eouts'. tlsimpl.
-          ssplit; reflexivity.
+      destruct repr; destruct a_valid0; destruct d_ready0;
+        tlsimpl; boolsimpl; subst.
+      all: try match goal with
+               | H: true = true -> _ |- _ =>
+                 destruct H; [auto|subst..]
+               end.
+      all: logical_simplify; subst; boolsimpl.
+      all: repeat eexists; cbn.
+      all: rewrite List.resize_noop by assumption.
+      all: change 1073741823 with (N.ones 30);
+        rewrite N.land_ones;
+        replace 4 with (2 ^ 2) by reflexivity;
+        rewrite <- ! N.shiftr_div_pow2;
+        try reflexivity.
     Qed.
 
     Existing Instances tlul_adapter_reg_invariant_at_reset tlul_adapter_reg_invariant_preserved
              tlul_adapter_reg_output_correct.
     Global Instance tlul_adapter_reg_correctness : correctness_for tlul_adapter_reg.
     Proof. constructor; typeclasses eauto. Defined.
-
-
-
-    Lemma outstanding_in_repr : forall r_tlul t,
-        outstanding_h2d r_tlul = Some t ->
-        In t r_tlul.
-    Proof.
-      intros ? ?.
-      induction r_tlul; intros Houts; cbn in Houts.
-      - discriminate.
-      - destruct (outstanding_h2d r_tlul) eqn:Houts'.
-        + destruct d_ready.
-          * discriminate.
-          * apply in_cons. auto.
-        + destruct (a_valid a).
-          * inversion Houts. apply in_eq.
-          * discriminate.
-    Qed.
-
-    Lemma outstanding_a_valid : forall r_tlul t,
-        outstanding_h2d r_tlul = Some t ->
-        a_valid t = true.
-    Proof.
-      intros ? ?.
-      induction r_tlul; intros Houts; cbn in Houts.
-      - discriminate.
-      - destruct (outstanding_h2d r_tlul) eqn:Houts'.
-        + destruct d_ready.
-          * discriminate.
-          * auto.
-        + destruct (a_valid a) eqn:Hvalid.
-          * inversion Houts. subst. assumption.
-          * discriminate.
-    Qed.
-
-    Lemma outstanding_prec : forall tl_st r_tlul t,
-        tlul_invariant tl_st r_tlul ->
-        outstanding_h2d r_tlul = Some t ->
-        a_opcode t = Get \/ a_opcode t = PutFullData.
-    Proof.
-      intros ? ? ? Hinvar Houts. simpl in *.
-      apply outstanding_in_repr in Houts as Hin.
-      unfold tlul_invariant in Hinvar. logical_simplify.
-      eapply Forall_forall in H. 2: apply Hin.
-      apply H.
-      eapply outstanding_a_valid.
-      apply Houts.
-    Qed.
-End TLULSpec.
+End TLSpec.
