firmware/IncrementWait/Incr.v
@@ -113,7 +113,7 @@ Section Var.
                     else `replace` registers' `K (sz:=1) 1` `K 1` in
 
            (busy', done', registers', tl_d2h') initially
-           (false, (false, ([0; 1], default (t:=tl_d2h_t))))
+           (false, (false, ([0; 1], set_a_ready true (default (t:=tl_d2h_t)))))
            : denote_type (Bit ** Bit ** Vec (BitVec 32) 2 ** tl_d2h_t)
         in
 
@@ -257,13 +257,47 @@ Section Spec.
   | RSBusy (data : N)
   | RSDone (res : N).
 
-  Definition repr := (repr_state * list N * list tl_h2d * inner_repr)%type.
+  Definition repr := (repr_state * repr_state * list N * TLUL.repr_state * inner_repr)%type.
 
   Global Instance incr_invariant : invariant_for incr repr :=
     fun (state : denote_type (state_of incr)) repr =>
       let '((s_busy, (s_done, (s_regs, s_d2h))), (s_tlul, s_inner)) := state in
-      let '(r_state, r_regs, r_tlul, r_inner) := repr in
-      tlul_invariant (reg_count:=2) s_tlul r_tlul
+      let '(r_state, r_prev_state, r_regs, r_tl, r_inner) := repr in
+      tlul_invariant (reg_count:=2) s_tlul r_tl
+      /\ match r_tl with
+        | TLUL.Idle =>
+          d_valid    s_d2h = false
+          /\ d_error  s_d2h = false
+          /\ a_ready  s_d2h = true
+        | TLUL.OutstandingAccessAckData h2d regs =>
+          d_valid    s_d2h = true
+          /\ d_opcode s_d2h = AccessAckData
+          /\ d_param  s_d2h = 0
+          /\ d_size   s_d2h = (a_size h2d)
+          /\ d_source s_d2h = (a_source h2d)
+          /\ d_sink   s_d2h = 0
+          /\ d_data   s_d2h = (List.nth (N.to_nat ((((a_address h2d) / 4) mod (2 ^ 30)))) regs 0%N)
+          /\ d_user   s_d2h = 0
+          /\ d_error  s_d2h = false
+          /\ a_ready  s_d2h = false
+          /\ match r_prev_state with
+            | RSIdle => nth 1 regs 0%N = 1
+            | RSBusy data => nth 1 regs 0%N = 2
+            | RSDone res => nth 0 regs 0%N = res
+                           /\ nth 1 regs 0%N = 4
+            end
+          (* /\ (exists input, update_repr (r_prev_state, ... ..) = r_state) *)
+        | TLUL.OutstandingAccessAck h2d  =>
+          d_valid    s_d2h = true
+          /\ d_opcode s_d2h = AccessAck
+          /\ d_param  s_d2h = 0
+          (* /\ d_size   s_d2h =  *)
+          /\ d_source s_d2h = (a_source h2d)
+          /\ d_sink   s_d2h = 0
+          /\ d_user   s_d2h = 0
+          /\ d_error  s_d2h = false
+          /\ a_ready  s_d2h = false
+        end
       /\ inner_invariant s_inner r_inner
       /\ match r_state with
         | RSIdle => s_busy = false /\ s_done = false
@@ -280,44 +314,43 @@ Section Spec.
       /\ s_regs = r_regs
       /\ length r_regs = 2%nat.
 
-  Existing Instance tlul_specification.
+  Existing Instance tl_specification.
 
   Instance incr_specification
     : specification_for incr repr :=
-    {| reset_repr := (RSIdle, [0; 1], [], IISIdle);
+    {| reset_repr := (RSIdle, RSIdle, [0; 1], TLUL.Idle, IISIdle);
 
        update_repr :=
          fun (input : denote_type (input_of incr)) repr =>
            let '(i_h2d, tt) := input in
-           let '(r_state, r_regs, r_tlul, r_inner) := repr in
+           let '(r_state, r_prev_state, r_regs, r_tl, r_inner) := repr in
 
            let h2d := set_a_address (N.land (a_address i_h2d) 4) i_h2d in
 
-           let r_tlul' :=
+           let r_tl' :=
                let tlul_input := (h2d, (r_regs, tt)) in
                update_repr (c:=tlul_adapter_reg (reg_count:=2))
-                           tlul_input r_tlul in
+                           tlul_input r_tl in
 
            (* compute (some) tlul output *)
            let '(is_read, is_write, address, write_data) :=
-               match outstanding_h2d (h2d :: r_tlul) with
-               | None => (false, false, 0, 0)
-               | Some h2d' =>
-                 if a_opcode h2d' =? Get then
-                   match outstanding_h2d r_tlul with
-                   | None => (a_valid h2d, false, a_address h2d, 0)
+               match r_tl' with
+               | TLUL.Idle => (false, false, 0, 0)
+               | TLUL.OutstandingAccessAckData _ _ =>
+                 match r_tl with
+                   | TLUL.Idle => (a_valid h2d, false, a_address h2d, 0)
                    | _ => (false, false, 0, 0)
-                   end
-                 else if a_opcode h2d' =? PutFullData then
-                   match outstanding_h2d r_tlul with
-                   | None => (false, a_valid h2d, a_address h2d, a_data h2d)
-                   | _ => (false, false, 0, 0)
-                   end
-                 else (false, false, 0, 0)
+                 end
+               | TLUL.OutstandingAccessAck _ =>
+                 match r_tl with
+                 | TLUL.Idle => (false, a_valid h2d, a_address h2d, a_data h2d)
+                 | _ => (false, false, 0, 0)
+                 end
                end in
 
            let r_inner' :=
-               let inner_input := (match r_state with RSIdle => is_write | _ => false end, (write_data, tt)) in
+               let inner_input := (match r_state with RSIdle => is_write | _ => false end,
+                                   (write_data, tt)) in
                update_repr (c:=inner) inner_input r_inner in
 
            let r_state' :=
@@ -346,12 +379,12 @@ Section Spec.
                | RSDone _ => replace 1 4 r_regs'
                end in
 
-           (r_state', r_regs', h2d :: r_tlul, r_inner');
+           (r_state', r_state, r_regs', r_tl', r_inner');
 
        precondition :=
          fun (input : denote_type (input_of incr)) repr =>
            let '(i_h2d, tt) := input in
-           let '(r_state, r_regs, r_tlul, r_inner) := repr in
+           let '(r_state, r_prev_state, r_regs, r_tl, r_inner) := repr in
 
            let h2d := set_a_address (N.land (a_address i_h2d) 4) i_h2d in
 
@@ -359,14 +392,15 @@ Section Spec.
 
            let prec_tlul :=
                precondition (tlul_adapter_reg (reg_count:=2))
-                            tlul_input r_tlul in
+                            tlul_input r_tl in
 
            let prec_inner :=
                forall d2h is_read is_write address write_data write_mask,
                  postcondition (tlul_adapter_reg (reg_count:=2))
-                               tlul_input r_tlul
+                               tlul_input r_tl
                                (d2h, (is_read, (is_write, (address, (write_data, write_mask)))))
-                 -> precondition inner (match r_state with RSIdle => is_write | _ => false end, (write_data, tt)) r_inner in
+                 -> precondition inner (match r_state with RSIdle => is_write | _ => false end,
+                                       (write_data, tt)) r_inner in
 
            prec_tlul /\ prec_inner;
 
@@ -374,7 +408,7 @@ Section Spec.
          fun (input : denote_type (input_of incr)) repr
            (output : denote_type (output_of incr)) =>
            let '(i_h2d, tt) := input in
-           let '(r_state, r_regs, r_tlul, r_inner) := repr in
+           let '(r_state, r_prev_state, r_regs, r_tl, r_inner) := repr in
 
            let h2d := set_a_address (N.land (a_address i_h2d) 4) i_h2d in
 
@@ -382,7 +416,7 @@ Section Spec.
                let tlul_input := (h2d, (r_regs, tt)) in
                exists req,
                  postcondition (tlul_adapter_reg (reg_count:=2))
-                               tlul_input r_tlul
+                               tlul_input r_tl
                                (output, req) in
            postc_tlul;
     |}.
@@ -390,206 +424,169 @@ Section Spec.
   Lemma incr_invariant_at_reset : invariant_at_reset incr.
   Proof.
     simplify_invariant incr.
-    cbn. ssplit; try reflexivity.
-    apply (tlul_adapter_reg_invariant_at_reset (reg_count:=2)).
+    cbn. ssplit; [apply (tlul_adapter_reg_invariant_at_reset (reg_count:=2))
+                 | reflexivity..].
   Qed.
 
   Existing Instance tlul_adapter_reg_correctness.
 
   Lemma incr_invariant_preserved : invariant_preserved incr.
   Proof.
-    intros (h2d, t) state (((r_state, r_regs), r_tlul), r_inner). destruct t.
+    intros (h2d, t) state ((((r_state, r_prev_state), r_regs), r_tl), r_inner). destruct t.
     cbn in * |-. destruct state as ((busy, (done, (registers, d2h))), (tl_st, inner_st)).
     destruct_tl_h2d. destruct_tl_d2h.
     intros repr' ? Hinvar Hprec; subst.
     simplify_invariant incr. logical_simplify. subst.
     simplify_spec incr. logical_simplify. subst.
     (* destruct Hprec as [regs Hprec]. *)
-    cbv [incr]. stepsimpl.
-    use_correctness.
     match goal with
-    | H: (match outstanding_h2d (_::r_tlul) with | _ => _ end) |- _ =>
-      rename H into Htl_postc
+    | |- context [step incr ?s ?i] =>
+      remember (step incr s i) as step eqn:Estep;
+        cbv -[Semantics.step inner tlul_adapter_reg] in Estep;
+          subst
     end.
+    stepsimpl.
+    use_correctness.
+    rename H9 into Hpostc_tl.
     repeat (destruct_pair_let; cbn [fst snd]).
     ssplit.
     - eapply tlul_adapter_reg_invariant_preserved.
       2: apply H.
       + reflexivity.
       + assumption.
+    - pose (r_tl_:=r_tl); destruct r_tl; logical_simplify; subst.
+      + clear H5.
+        destruct_tl_h2d; destruct_tl_d2h; tlsimpl; subst.
+        pose (r_state_:=r_state); destruct r_state; cbn in *; logical_simplify; subst;
+          pose (a_valid_:=a_valid); (destruct a_valid;
+                                     [ match goal with
+                                       | H: true = true -> _ |- _ =>
+                                         destruct H; [auto|subst..]
+                                       end|]); cbn in *; logical_simplify; subst;
+            ssplit; auto.
+      + clear H5.
+        destruct_tl_h2d; destruct_tl_d2h; tlsimpl; subst.
+        pose (r_state_:=r_state); destruct r_state; cbn in *; logical_simplify; subst;
+          pose (d_ready_:=d_ready); destruct d_ready; cbn in *; logical_simplify; subst;
+            ssplit; auto.
+      + clear H5.
+        destruct_tl_h2d; destruct_tl_d2h; tlsimpl; subst.
+        pose (r_state_:=r_state); destruct r_state; cbn in *; logical_simplify; subst;
+          pose (d_ready_:=d_ready); destruct d_ready; cbn in *; logical_simplify; subst;
+            ssplit; reflexivity.
     - eapply inner_invariant_preserved.
-      2: apply H0.
+      2: eassumption.
       + simpl in *.
         destruct r_inner; try reflexivity.
-        destruct (outstanding_h2d r_tlul) eqn:Houts.
-        * destruct d_ready; logical_simplify; subst.
-          -- boolsimpl. destruct r_state; reflexivity.
-          -- eapply outstanding_prec in H as Hprec_t. 2: apply Houts.
-             destruct Hprec_t as [Hprec_t|Hprec_t];
-               rewrite Hprec_t in *; cbn in Htl_postc |- *; logical_simplify; subst;
-                 boolsimpl; destruct r_state; reflexivity.
+        destruct r_tl eqn:Houts; logical_simplify; subst.
         * destruct a_valid eqn:Hvalid; logical_simplify; subst.
-          -- cbn in Htl_postc.
-             match goal with
+          -- match goal with
              | H: true = true -> _ |- _ =>
                destruct H; try reflexivity; subst
-             end; cbn in Htl_postc; logical_simplify; subst;
+             end; logical_simplify; subst;
                boolsimpl; destruct r_state; logical_simplify; subst;
-                 reflexivity.
+                 cbn in Hpostc_tl |- *; logical_simplify; subst; reflexivity.
           -- boolsimpl; destruct r_state; reflexivity.
-      + match goal with
-        | H: context [_ -> precondition inner _ r_inner] |- _ =>
-          eapply H
-        end.
-        do 8 eexists. ssplit.
-        1-2: reflexivity.
-        apply Htl_postc.
+
+        * destruct d_ready; logical_simplify; subst;
+            boolsimpl; destruct r_state; reflexivity.
+        * destruct d_ready; logical_simplify; subst;
+            boolsimpl; destruct r_state; reflexivity.
+      + simplify_spec inner. auto.
     - match goal with
       | H: context [_ -> precondition inner _ r_inner] |- _ => clear H
       end.
-      destruct r_inner; destruct r_state; destruct inner_st;
-        unfold inner_invariant in H0; logical_simplify; subst;
-          try discriminate;
-          try (destruct H4; discriminate).
-      all: destruct (outstanding_h2d r_tlul) eqn:Houts;
-        cbn [outstanding_h2d] in Htl_postc |- *; rewrite Houts in Htl_postc |- *.
-      all: tlsimpl; destruct d_ready; logical_simplify; subst; boolsimpl.
-      all: cbn; try (ssplit; try reflexivity;
-                     destruct x0 as [|? [|]]; try discriminate H3; reflexivity).
-      all: try (eapply outstanding_prec in H;
-                try match goal with
-                    | H: outstanding_h2d _ = Some _ |- outstanding_h2d _ = Some _ =>
-                      apply H
-                    end; destruct H; rewrite H in Htl_postc |- *; cbn in Htl_postc |- *;
-                logical_simplify; subst; ssplit;
-                try (left; reflexivity);
-                try (right; reflexivity);
-                try reflexivity;
-                destruct x0 as [|? [|]]; try discriminate H3; reflexivity).
-      all: try (destruct a_valid; simplify_spec (tlul_adapter_reg (reg_count:=2));
-                   logical_simplify; tlsimpl;
-                try match goal with
-                    | H: true = true -> _ |- _ =>
-                      destruct H; try reflexivity; subst
-                    end; try cbn in Htl_postc; logical_simplify; subst; cbn; ssplit;
-                try eexists;
-                try reflexivity;
-                destruct x0 as [|? [|]]; try discriminate H3; reflexivity).
-      all: try (destruct a_valid; ssplit;
-                try (left; reflexivity);
-                try (right; reflexivity);
-                try reflexivity;
-                destruct x0 as [|? [|]]; try discriminate H3; reflexivity).
-      all: try (destruct a_valid; simplify_spec (tlul_adapter_reg (reg_count:=2));
-                tlsimpl; logical_simplify;
-                try match goal with
-                    | H: true = true -> _ |- _ =>
-                      destruct H; try reflexivity; subst
-                    end; try cbn in Htl_postc; logical_simplify; subst;
-                boolsimpl; destruct (negb (N.land a_address 4 =? 0)) eqn:Haddr;
-                cbn; try (rewrite Haddr); ssplit;
-                try (left; reflexivity);
-                try (right; reflexivity);
-                try reflexivity;
-                destruct x0 as [|? [|]]; try discriminate H3; reflexivity).
-      all: try (inversion H5; subst; clear H5;
-            destruct x as [|[|[|?]]]; cbn; ssplit;
-            try eexists;
-            try (left; reflexivity);
-            try (right; reflexivity);
-            try reflexivity;
-            try (destruct x0 as [|? [|]]; try discriminate H3; reflexivity);
-            exfalso; lia).
-      all: destruct H5; discriminate.
+      destruct r_tl; destruct r_inner; destruct r_state; destruct inner_st;
+        logical_simplify; subst.
+      all: simplify_invariant inner.
+      all: try discriminate.
+      all: simplify_spec (tlul_adapter_reg (reg_count:=2)); logical_simplify; tlsimpl; subst.
+      all: destruct a_valid; [destruct H3; subst|]; cbn in Hpostc_tl; logical_simplify; subst; cbn.
+      all: eauto.
+      all: try (destruct (negb (N.land a_address 4 =? 0)) eqn:Haddr;
+               ssplit; eauto;
+               destruct x0 as [|? [|]]; cbn in *; try discriminate; reflexivity).
+      all: try (destruct count as [|[|[|]]]; [lia|..|lia]; cbn;
+             ssplit; eauto;
+             destruct x0 as [|? [|]]; cbn in *; try discriminate; reflexivity).
+      all: try (destruct H6; discriminate).
+      all: try (destruct d_ready; logical_simplify; subst; cbn;
+                  ssplit; eauto;
+                  destruct x0 as [|? [|]]; cbn in *; try discriminate; reflexivity).
     - match goal with
       | H: context [_ -> precondition inner _ r_inner] |- _ => clear H
       end.
-      destruct r_inner; destruct r_state; destruct inner_st;
-        unfold inner_invariant in H0; logical_simplify; subst;
-          try discriminate.
-      all: destruct (outstanding_h2d r_tlul) eqn:Houts;
-        cbn [outstanding_h2d] in Htl_postc |- *; rewrite Houts in Htl_postc |- *.
-      all: tlsimpl; destruct d_ready; logical_simplify; subst; boolsimpl.
-      all: try reflexivity.
-      all: try (destruct H5; discriminate).
-      all: try (inversion H5; subst; clear H5;
-            destruct x as [|[|[|?]]]; try reflexivity; exfalso; lia).
-      all: try (eapply outstanding_prec in H;
-                try match goal with
-                    | H: outstanding_h2d _ = Some _ |- outstanding_h2d _ = Some _ =>
-                      apply H
-                    end; destruct H; rewrite H in Htl_postc |- *; cbn in Htl_postc |- *;
-                logical_simplify; subst; cbn; reflexivity).
-      all: try (destruct a_valid; simplify_spec (tlul_adapter_reg (reg_count:=2));
-                tlsimpl; logical_simplify;
-                try match goal with
-                    | H: true = true -> _ |- _ =>
-                      destruct H; try reflexivity; subst
-                    end; try cbn in Htl_postc; logical_simplify; subst; reflexivity).
-      all: try (destruct a_valid; simplify_spec (tlul_adapter_reg (reg_count:=2));
-                tlsimpl; logical_simplify;
-                try match goal with
-                    | H: true = true -> _ |- _ =>
-                      destruct H; try reflexivity; subst
-                    end; try cbn in Htl_postc; logical_simplify; subst;
-                boolsimpl; destruct (negb (N.land a_address 4 =? 0)) eqn:Haddr;
-                cbn; try (rewrite Haddr); reflexivity).
-    - all: match goal with
-           | |- length (match ?v with _ => _ end) = 2%nat => destruct v
-           end;
-        match goal with
-        | |- context [update_repr ?ui ?ur] =>
-          remember (update_repr (c:=inner) ui ur) as up eqn:?H;
-            replace (update_repr (c:=inner) ui ur) with up;
-            destruct up
-        end;
-        rewrite ! length_replace; assumption.
+      destruct r_tl; destruct r_inner; destruct r_state; destruct inner_st;
+        logical_simplify; subst.
+      all: simplify_invariant inner.
+      all: try discriminate.
+      all: simplify_spec (tlul_adapter_reg (reg_count:=2)); logical_simplify; tlsimpl; subst.
+      all: destruct a_valid; [destruct H3; subst|]; cbn in Hpostc_tl; logical_simplify; subst; cbn.
+      all: eauto.
+      all: try (destruct (negb (N.land a_address 4 =? 0)) eqn:Haddr;
+               ssplit; eauto;
+               destruct x0 as [|? [|]]; cbn in *; try discriminate; reflexivity).
+      all: try (destruct count as [|[|[|]]]; [lia|..|lia]; cbn;
+             ssplit; eauto;
+             destruct x0 as [|? [|]]; cbn in *; try discriminate; reflexivity).
+      all: try (destruct H6; discriminate).
+      all: try (destruct d_ready; logical_simplify; subst; cbn;
+                  ssplit; eauto;
+                  destruct x0 as [|? [|]]; cbn in *; try discriminate; reflexivity).
+    - repeat destruct_one_match; rewrite ! length_replace; assumption.
   Qed.
 
   Lemma incr_output_correct : output_correct incr.
   Proof.
-    intros (h2d, t) state (((r_state, r_regs), r_tlul), r_inner). destruct t.
-    cbn in * |-. destruct state as ((busy, (done, (registers, d2h))), (tl_st, inner_st)).
-    destruct_tl_h2d. destruct_tl_d2h.
-    intros Hinvar Hprec; subst.
-    simplify_invariant incr. logical_simplify. subst.
-    simplify_spec incr. logical_simplify. subst.
-    cbv [incr]. stepsimpl.
-    use_correctness.
-    match goal with
-    | H: (match outstanding_h2d (_::r_tlul) with | _ => _ end) |- _ =>
-      rename H into Htl_postc
-    end.
-    repeat (destruct_pair_let; cbn [fst snd]).
-    tlsimpl.
-    destruct r_inner; destruct r_state; destruct inner_st;
-      unfold inner_invariant in H0; logical_simplify; subst;
-        try discriminate;
-        try (destruct H5; discriminate).
-    all: destruct (outstanding_h2d r_tlul) eqn:Houts;
-      cbn [outstanding_h2d] in Htl_postc |- *; rewrite Houts in Htl_postc |- *.
-    all: tlsimpl; destruct d_ready; logical_simplify; subst; boolsimpl.
-    all: do 9 eexists.
-    all: ssplit; try reflexivity; tlsimpl; ssplit; try reflexivity; try assumption.
-    all: try (eapply outstanding_prec in H;
-              try match goal with
-                  | H: outstanding_h2d _ = Some _ |- outstanding_h2d _ = Some _ =>
-                    apply H
-                  end; destruct H; rewrite H in Htl_postc |- *; cbn in Htl_postc |- *;
-              logical_simplify; subst; ssplit;
-              try (left; reflexivity);
-              try (right; reflexivity);
-              try assumption;
-              reflexivity).
-    all: try (destruct a_valid; simplify_spec (tlul_adapter_reg (reg_count:=2));
-              tlsimpl; destruct H2;
-              try match goal with
-                  | H: true = true -> _ |- _ =>
-                    destruct H; try reflexivity; subst
-                  end; cbn in Htl_postc; logical_simplify; subst; cbn; ssplit;
-              try eexists; try assumption; reflexivity).
-    Unshelve. all: auto.
-  Qed.
+  Admitted.
+  (*   intros (h2d, t) state (((r_state, r_regs), r_tl), r_inner). destruct t. *)
+  (*   cbn in * |-. destruct state as ((busy, (done, (registers, d2h))), (tl_st, inner_st)). *)
+  (*   destruct_tl_h2d. destruct_tl_d2h. *)
+  (*   intros Hinvar Hprec; subst. *)
+  (*   simplify_invariant incr. logical_simplify. subst. *)
+  (*   simplify_spec incr. logical_simplify. subst. *)
+  (*   match goal with *)
+  (*   | |- context [step incr ?s ?i] => *)
+  (*     remember (step incr s i) as step eqn:Estep; *)
+  (*       cbv -[Semantics.step inner tlul_adapter_reg] in Estep; *)
+  (*         subst *)
+  (*   end. *)
+  (*   stepsimpl. *)
+  (*   use_correctness. *)
+  (*   match goal with *)
+  (*   | H: (match outstanding_h2d (_::r_tl) with | _ => _ end) |- _ => *)
+  (*     rename H into Htl_postc *)
+  (*   end. *)
+  (*   repeat (destruct_pair_let; cbn [fst snd]). *)
+  (*   tlsimpl. *)
+  (*   destruct r_inner; destruct r_state; destruct inner_st; *)
+  (*     unfold inner_invariant in H0; logical_simplify; subst; *)
+  (*       try discriminate; *)
+  (*       try (destruct H5; discriminate). *)
+  (*   all: destruct (outstanding_h2d r_tl) eqn:Houts; *)
+  (*     cbn [outstanding_h2d] in Htl_postc |- *; rewrite Houts in Htl_postc |- *. *)
+  (*   all: tlsimpl; destruct d_ready; logical_simplify; subst; boolsimpl. *)
+  (*   all: do 9 eexists. *)
+  (*   all: ssplit; try reflexivity; tlsimpl; ssplit; try reflexivity; try assumption. *)
+  (*   all: try (eapply outstanding_prec in H; *)
+  (*             try match goal with *)
+  (*                 | H: outstanding_h2d _ = Some _ |- outstanding_h2d _ = Some _ => *)
+  (*                   apply H *)
+  (*                 end; destruct H; rewrite H in Htl_postc |- *; cbn in Htl_postc |- *; *)
+  (*             logical_simplify; subst; ssplit; *)
+  (*             try (left; reflexivity); *)
+  (*             try (right; reflexivity); *)
+  (*             try assumption; *)
+  (*             reflexivity). *)
+  (*   all: try (destruct a_valid; simplify_spec (tlul_adapter_reg (reg_count:=2)); *)
+  (*             tlsimpl; destruct H2; *)
+  (*             try match goal with *)
+  (*                 | H: true = true -> _ |- _ => *)
+  (*                   destruct H; try reflexivity; subst *)
+  (*                 end; cbn in Htl_postc; logical_simplify; subst; cbn; ssplit; *)
+  (*             try eexists; try assumption; reflexivity). *)
+  (*   Unshelve. all: auto. *)
+  (* Qed. *)
 
   Existing Instances incr_invariant_at_reset incr_invariant_preserved
            incr_output_correct.
