firmware/IncrementWait/CavaIncrementDevice.v
@@ -34,47 +34,96 @@ Import ListNotations.
 Section WithParameters.
   Instance var : tvar := denote_type.
 
+  Existing Instance Incr.inner_specification.
+  Existing Instance Incr.inner_correctness.
+  Existing Instance Incr.inner_invariant.
+
+  Existing Instance TLUL.tl_specification.
+  Existing Instance TLUL.tlul_invariant.
+  Existing Instance TLUL.tlul_adapter_reg_correctness.
+
+  Existing Instance incr_specification.
+  Existing Instance incr_invariant.
+  Existing Instance incr_correctness.
+
   Context {word: Interface.word 32} {word_ok: word.ok word}
           {Mem: map.map word byte} {Registers: map.map Z word}.
 
   Global Instance counter_device: device := {|
     device.state := denote_type (state_of incr);
-    device.is_ready_state s := exists r_regs r_tlul r_inner,
-        incr_invariant s (RSIdle, r_regs, r_tlul, r_inner);
-    device.run1 s i := Semantics.step incr s (i, tt);
+    device.is_ready_state s := exists r_prev_state r_regs r_inner,
+        incr_invariant s (RSIdle, r_prev_state, r_regs, TLUL.Idle, r_inner);
+    device.last_d2h '((_, (_, (_, d2h))), _) := d2h;
+    device.tl_inflight_ops '((_, (_, (_, d2h))), _) :=
+      if d_valid d2h then [d_source d2h] else [];
+    device.run1 s i := fst (Semantics.step incr s (i, tt));
     device.addr_range_start := INCR_BASE_ADDR;
     device.addr_range_pastend := INCR_END_ADDR;
-    device.maxRespDelay '((istate, (val, tl_d2h)), tlul_state) h2d :=
-      (* if the value register was requested, and we're in state Busy1, it will take one
-         more cycle to respond, else we will respond immediately *)
-      if ((a_address h2d mod 8 =? 0(*register address=VALUE*))%N && (istate =? 1 (*Busy1*))%N)%bool
-      then 1%nat else 0%nat;
+    device.maxRespDelay '((_, (_, (_, d2h))), _) :=
+      if a_ready d2h then 2
+      else if d_valid d2h then 1
+           else 0;
+    (* The last [else] is not reachable, because [d_valid] is always the
+       negation of [a_ready]. *)
   |}.
 
   (* conservative upper bound matching the instance given in IncrementWaitToRiscv *)
   Global Instance circuit_spec : circuit_behavior :=
   {| ncycles_processing := 15%nat |}.
 
-  Inductive counter_related_spec: IncrementWaitSemantics.state -> repr -> Prop :=
-  | IDLE_related: forall r_regs r_tl r_inner,
-      counter_related_spec IDLE (RSIdle, r_regs, r_tl, r_inner)
-  | BUSY_related: forall r_regs r_tl r_inner val ncycles,
+
+  Inductive counter_related_base: IncrementWaitSemantics.state -> Incr.repr_state -> Incr.inner_state -> Prop :=
+  | IDLE_related: forall r_innr,
+      counter_related_base IDLE RSIdle r_innr
+  | BUSY1_related: forall val ncycles,
+      (1 < ncycles)%nat ->
+      counter_related_base (BUSY val ncycles) (RSBusy (word_to_N val))
+                           (IISBusy (word_to_N val) 1)
+  | BUSY2_related: forall val ncycles,
       (0 < ncycles)%nat ->
-      counter_related_spec (BUSY val ncycles)
-                           (RSBusy (word_to_N val), r_regs, r_tl, r_inner)
+      counter_related_base (BUSY val ncycles) (RSBusy (word_to_N val))
+                           (IISBusy (word_to_N val) 2)
   (* the hardware is already done, but the software hasn't polled it yet to find out,
      so we have to relate a software-BUSY to a hardware-done: *)
-  | BUSY_done_related: forall r_regs r_tl r_inner val ncycles,
-      counter_related_spec (BUSY val ncycles)
-                           (RSDone (word_to_N (word.add (word.of_Z 1) val)), r_regs, r_tl, r_inner)
-  | DONE_related: forall r_regs r_tl r_inner val,
-      nth 0 r_regs 0%N = (word_to_N val)
-      -> counter_related_spec (DONE val)
-                             (RSDone (word_to_N val), r_regs, r_tl, r_inner).
+  | BUSY_done_related: forall val ncycles r_innr,
+      counter_related_base (BUSY val ncycles) (RSDone (word_to_N (word.add (word.of_Z 1) val))) r_innr
+  | DONE_related: forall val r_innr,
+      counter_related_base (DONE val) (RSDone (word_to_N val)) r_innr.
 
-  Definition counter_related (sH : IncrementWaitSemantics.state)
-             (sL : denote_type (state_of incr)) : Prop :=
-    exists repr, counter_related_spec sH repr /\ incr_invariant sL repr.
+  Inductive counter_related_spec: IncrementWaitSemantics.state -> repr ->
+                                  list tl_h2d -> Prop :=
+  | No_inflight: forall sH r_state r_prev_state r_regs r_inner,
+      counter_related_base sH r_state r_inner ->
+      counter_related_spec sH (r_state, r_prev_state, r_regs, TLUL.Idle, r_inner) []
+  | Inflight_read_status: forall sH r_state r_prev_state r_regs r_tl r_tl_regs r_inner h2d,
+      counter_related_base sH r_state r_inner ->
+      r_tl = TLUL.OutstandingAccessAckData (set_a_address 4 h2d) r_tl_regs ->
+      a_valid h2d = true ->
+      a_opcode h2d = Get ->
+      a_address h2d = word_to_N (state_machine.reg_addr STATUS) ->
+      counter_related_spec sH (r_state, r_prev_state, r_regs, r_tl, r_inner) [h2d]
+  | Inflight_read_value: forall r_prev_state r_regs r_tl r_tl_regs r_inner val h2d,
+      r_tl = TLUL.OutstandingAccessAckData (set_a_address 0 h2d) r_tl_regs ->
+      nth 0 r_tl_regs 0%N = word_to_N val ->
+      a_valid h2d = true ->
+      a_opcode h2d = Get ->
+      a_address h2d = word_to_N (state_machine.reg_addr VALUE) ->
+      counter_related_spec (DONE val)
+                           (RSIdle, r_prev_state, r_regs, r_tl, r_inner)
+                           [h2d]
+  | Inflight_write_value: forall r_prev_state r_regs r_tl r_inner val h2d,
+      r_tl = TLUL.OutstandingAccessAck (set_a_address 0 h2d) ->
+      a_valid h2d = true ->
+      a_opcode h2d = PutFullData ->
+      a_address h2d = word_to_N (state_machine.reg_addr VALUE) ->
+      a_data h2d = (word_to_N val) ->
+      counter_related_spec (IDLE)
+                           (RSBusy (word_to_N val), r_prev_state, r_regs, r_tl, r_inner)
+                           [h2d].
+
+  Definition counter_related {invariant : invariant_for incr repr} (sH : IncrementWaitSemantics.state)
+             (sL : denote_type (state_of incr)) (inflight_h2ds : list tl_h2d) : Prop :=
+    exists repr, counter_related_spec sH repr inflight_h2ds /\ invariant sL repr.
 
   (* This should be in bedrock2.ZnWords. It is use by ZnWords, which is used in
      the two following Lemmas. *)
@@ -104,162 +153,81 @@ Section WithParameters.
       eapply pair_equal_spec in H; destruct H as [?H0 ?H1]
     end.
 
-  (* Ltac destruct_tlul_adapter_reg_state := *)
-  (*   match goal with *)
-  (*   | H : N * (N * (N * (bool * (bool * (bool * bool))))) |- _ => *)
-  (*     destruct H as [?reqid [?reqsz [?rspop [?error [?outstanding [?we_o ?re_o]]]]]] *)
-  (*   end. *)
-
   Lemma N_to_word_word_to_N: forall v, N_to_word (word_to_N v) = v.
   Proof. intros. unfold N_to_word, word_to_N. ZnWords. Qed.
 
-  Existing Instance Incr.inner_specification.
-  Existing Instance Incr.inner_correctness.
-  Existing Instance Incr.inner_invariant.
+(* TODO move to coqutil *)
+Ltac contradictory H :=
+  lazymatch type of H with
+  | ?x <> ?x => exfalso; apply (H eq_refl)
+  | False => case H
+  end.
 
-  Existing Instance TLUL.tlul_specification.
-  Existing Instance TLUL.tlul_adapter_reg_correctness.
-  Existing Instance TLUL.tlul_invariant.
+Require Import coqutil.Tactics.autoforward.
 
-  Existing Instance incr_specification.
-  Existing Instance incr_correctness.
+Ltac fwd_step ::=
+  match goal with
+  | H: ?T |- _ => is_destructible_and T; destr_and H
+  | H: exists y, _ |- _ => let yf := fresh y in destruct H as [yf H]
+  | H: ?x = ?x |- _ => clear H
+  | H: True |- _ => clear H
+  | H: ?LHS = ?RHS |- _ =>
+    let h1 := head_of_app LHS in is_constructor h1;
+    let h2 := head_of_app RHS in is_constructor h2;
+    (* if not eq, H is a contradiction, but we don't want to change the number
+       of open goals in this tactic *)
+    constr_eq h1 h2;
+    (* we don't use `inversion H` or `injection H` because they unfold definitions *)
+    inv_rec LHS RHS;
+    clear H
+  | E: ?x = ?RHS |- context[match ?x with _ => _ end] =>
+    let h := head_of_app RHS in is_constructor h; rewrite E in *
+  | H: context[match ?x with _ => _ end], E: ?x = ?RHS |- _ =>
+    let h := head_of_app RHS in is_constructor h; rewrite E in *
+  | H: context[match ?x with _ => _ end] |- _ =>
+    (* note: recursive invocation of fwd_step for contradictory cases *)
+    destr x; try solve [repeat fwd_step; contradictory H]; []
+  | H: _ |- _ => autoforward with typeclass_instances in H
+  | |- _ => progress subst
+  | |- _ => progress fwd_rewrites
+  end.
 
-  Lemma runUntilResp_big_step : forall s h2d repr,
-      precondition incr (h2d, tt) repr
-      -> a_valid h2d = true
-      -> d_ready h2d = true (* TODO: do we need this? *)
-      -> incr_invariant s repr
-      -> exists n inputs s' repr' d2h s'',
-          device.runUntilResp h2d device.maxRespDelay s = (Some d2h, s'')
-          /\ n <= device.maxRespDelay
-          /\ inputs = repeat (h2d, tt) n
-          /\ s' = snd (simulate' incr inputs s)
-          (* /\ (s'', d2h) = Semantics.step incr s' (h2d, tt) *)
-          /\ repr' = fold_left (fun r i => update_repr (c:=incr) i r) inputs repr
-          (* /\ invariant s' repr' *)
-          /\ postcondition incr (h2d, tt) repr' d2h
-          /\ d_valid d2h = true
-          /\ incr_invariant s'' (update_repr (c:=incr) (h2d, tt) repr').
-  Proof.
-    intros ? ? ? Hprec Ea_valid Ed_ready Hinv.
-    unfold device.maxRespDelay, device.runUntilResp, device.state, device.run1, counter_device,
-    state_machine.read_step, increment_wait_state_machine, read_step in *.
-    eapply output_correct_pf in Hinv as Houtput.
-    apply Houtput in Hprec as Hpostc. clear Houtput.
-    cbn in s, h2d. destruct_tl_h2d.
-    destruct repr as (((?r_state, ?r_regs), ?r_tl), ?r_inner).
-    assert (Hprec_temp := Hprec).
-    unfold precondition, incr_specification in Hprec_temp.
-    logical_simplify.
-    unfold precondition, tlul_specification in H.
-    logical_simplify. tlsimpl. subst.
-    unfold postcondition, incr_specification in Hpostc.
-    unfold postcondition, tlul_specification in Hpostc.
-    destruct Hpostc as [[is_read [is_write [address [w_val w_mask]]]] [h2d' [regs' [d2h' [is_read' [is_write' [address' [w_val' [w_mask' Hpostc]]]]]]]]].
-    destruct_tl_h2d. destruct_tl_d2h. tlsimpl.
-    destruct Hpostc as [Hpostc1 [Hpostc2 Hpostc3]].
-    subst.
-    apply pair_equal_spec in Hpostc2.
-    logical_simplify.
-    cbn [outstanding_h2d] in Hpostc3.
-    destruct (outstanding_h2d r_tl) eqn:Eouts.
-    - cbn in Hpostc3. logical_simplify. subst.
-      assert (Hprec':
-                precondition incr
-                             (true,
-                              (a_opcode0,
-                               (a_param0, (a_size0, (a_source0, (a_address, (a_mask0, (a_data0, (a_user0, true)))))))), tt)
-                             (update_repr (c:=incr)
-                                          (true,
-                                           (a_opcode0,
-                                            (a_param0, (a_size0, (a_source0, (a_address, (a_mask0, (a_data0, (a_user0, true)))))))), tt)
-                                          (r_state, regs', r_tl, r_inner))).
-      { simplify_spec incr.
-        cbn [outstanding_h2d]. rewrite Eouts.
-        tlsimpl. ssplit.
-        - simplify_spec (tlul_adapter_reg (reg_count:=2)). tlsimpl. split; [|assumption].
-          match goal with
-          | |- context [length (match ?m with | _=> _ end)] =>
-            destruct m
-          end;
-          match goal with
-          | |- context [replace _ _ (match ?m with | _=> _ end)] =>
-            destruct m
-          end; rewrite ! length_replace; assumption.
-        - simplify_spec Incr.inner. intros. apply I.
-      }
-      destruct H1; [auto|..]; subst.
-      all: exists 1.
-      all: destruct_pair_let;
-        match goal with
-        | |- context [if d_valid ?c then _ else _] =>
-          match type of H2 with
-          | _ = ?r => replace c with r
-          end
-        end.
-      all: tlsimpl;
-        assert (Hinv' := Hprec);
-        eapply incr_invariant_preserved in Hinv;
-        [apply Hinv in Hinv'|reflexivity]; clear Hinv.
-      all: eapply output_correct_pf in Hinv' as Houtput';
-        apply Houtput' in Hprec' as Hpostc'; clear Houtput';
-          assert (Hpostc'' := Hpostc');
-        unfold postcondition, incr_specification in Hpostc';
-        unfold postcondition, tlul_specification in Hpostc';
-        cbn [update_repr outstanding_h2d] in Hpostc';
-        rewrite Eouts in Hpostc'; cbn -[Semantics.step] in Hpostc';
-        destruct Hpostc' as [[is_read [is_write [address [w_val w_mask]]]] [h2d' [regs'' [d2h' [is_read' [is_write' [address'' [w_val'' [w_mask'' Hpostc']]]]]]]]].
-      all: destruct_tl_h2d; destruct_tl_d2h; tlsimpl;
-        destruct Hpostc' as [Hpostc1' [Hpostc2' Hpostc3']];
-        subst;
-        apply pair_equal_spec in Hpostc2';
-        logical_simplify;
-        rewrite Eouts in Hpostc3';
-        tlsimpl.
-      all: cbn in Hpostc3'; logical_simplify; subst.
-      all: do 5 eexists; ssplit; try reflexivity.
-      1,5: destruct_pair_let;
-                match goal with
-        | |- context [if d_valid ?c then _ else _] =>
-          match type of H1 with
-          | _ = ?r => replace c with r
-          end
-        end; tlsimpl; reflexivity.
-      1,4: cbn [repeat fold_left];
-        match goal with
-        | H: postcondition incr _ _ ?c |- _ =>
-          match type of H1 with
-          | _ = ?r => replace c with r in H; apply H
-          end
-        end.
-      1,3: reflexivity.
-      1,2: cbn [repeat fold_left];
-        eapply incr_invariant_preserved; [reflexivity|assumption..].
-    - destruct H1; [auto|..]; subst; cbn in Hpostc3; logical_simplify; subst.
-      all: exists 0.
-      all: do 5 eexists; ssplit; try reflexivity; try lia.
-      1,5: destruct_pair_let;
-        match goal with
-        | |- context [if d_valid ?c then _ else _] =>
-          match type of H2 with
-          | _ = ?r => replace c with r
-          end
-        end; tlsimpl; reflexivity.
-      1,4: cbn [repeat fold_left];
-        eapply output_correct_pf in Hinv as Houtput;
-        apply Houtput in Hprec;
-        match goal with
-        | H: postcondition incr _ _ ?c |- _ =>
-          match type of H2 with
-          | _ = ?r => replace c with r in H; apply H
-          end
-        end.
-      1,3: reflexivity.
-      1,2: cbn [repeat fold_left];
-        eapply incr_invariant_preserved; [reflexivity|assumption..].
-  Qed.
+  Axiom TODO: False.
 
-  (* Set Printing All. *)
+  Ltac use_spec :=
+    match goal with
+    | Hrun: device.run1 ?sL ?input = ?sL',
+            Hinv: incr_invariant ?sL ?repr
+      |- _ =>
+      assert (Hprec: precondition incr (input, tt) repr);
+      [|
+       (* pose proof (output_correct_pf (c:=incr) (input, tt) sL repr Hinv Hprec) as Hpostc. *)
+       remember (update_repr (c:=incr) (input, tt) repr) as repr' eqn:Erepr';
+       pose proof (invariant_preserved_pf (c:=incr) (input, tt) sL repr repr' Erepr' Hinv Hprec) as Hinv';
+       unfold device.run1, counter_device in Hrun;
+       match type of Hrun with
+       | fst ?step = _ =>
+         remember step as res eqn:Hstep;
+         destruct res as (?sL'' & ?d2h);
+         cbn in Hrun; subst sL''; clear Hstep
+       end;
+       cbn [fst] in Hinv']
+    end.
+
+  Ltac inversion_rel_spec :=
+    match goal with
+    | H: counter_related_spec _ _ _ |- _ => inversion H; subst
+    end.
+  Ltac inversion_rel_base :=
+    match goal with
+    | H: counter_related_base _ _ _ |- _ => inversion H; subst
+    end.
+
+  (* Lemma output_last_d2h : forall s h2d s' d2h, *)
+  (*     (s', d2h) = Semantics.step incr s (h2d, tt) -> *)
+  (*     device.last_d2h s' = d2h. *)
+  (* Proof. *)
+
   Global Instance cava_counter_satisfies_state_machine:
     device_implements_state_machine counter_device increment_wait_state_machine.
   Proof.
@@ -267,194 +235,323 @@ Section WithParameters.
     - (* mmioAddrs_match: *)
       reflexivity.
     - (* initial_state_is_ready_state: *)
-      intros ? ? Hinit Hrel.
+      intros ? ? ? Hrel.
       cbn in *. subst. destruct Hrel as [?repr [?Hrel ?Hinv]].
-      inversion Hrel. subst.
-      do 3 eexists. eapply Hinv.
+      inversion_rel_spec. inversion_rel_base.
+      repeat eexists. eapply Hinv.
     - (* initial_states_are_related: *)
-      intros ? ? Hinit Hready.
-      cbn in *. destruct Hready as (?r_regs & ?r_tl & ?r_inner & ?Hinv). subst.
+      intros ? ? ? Hready.
+      cbn in *. destruct Hready as (?r_prev_state & ?r_regs & ?r_inner & ?Hinv). subst.
       unfold counter_related. eexists. split; [|apply Hinv].
-      apply IDLE_related.
+      apply No_inflight, IDLE_related.
     - (* initial_state_exists: *)
       intros ? Hready.
-      cbn in *. destruct Hready as (?r_regs & ?r_tl & ?r_inner & ?Hinv).
+      cbn in *. destruct Hready as (?r_prev_state & ?r_regs & ?r_inner & ?Hinv).
       eexists. split; [reflexivity|].
       unfold counter_related. eexists. split; [|apply Hinv].
-      apply IDLE_related.
+      apply No_inflight, IDLE_related.
     - (* nonMMIO_device_step_preserves_state_machine_state: *)
-      intros ? ? ? ? ? Ha_valid Hrel.
-      (* cbn in sL1, sL2. *)
-      (* destruct sL2 as ((?busy, (?done, (?regs, ?d2h))), (?s_tl, ?s_inner)). *)
-      (* destruct_tl_h2d. destruct_tl_d2h. tlsimpl. subst. *)
-      unfold device.run1. unfold counter_device.
-      intros Hstep.
-      destruct Hrel as [?repr [?Hrel ?Hinv]].
-      assert (Hprec: precondition incr (h2d, tt) repr).
+      intros ? ? ? ? Ha_valid [repr [Hrel Hinv]] **.
+      use_spec.
       { destruct_tl_h2d. destruct_tl_d2h. tlsimpl.
         cbn in sL1; destruct sL1 as ((?busy, (?done, (?regs, ?d2h))), (?s_tl, ?s_inner)).
-        destruct repr as (((?r_state, ?r_regs), ?r_tl), ?r_inner).
+        destruct repr as ((((?r_state, ?r_prev_state), ?r_regs), ?r_tl), ?r_inner).
         simplify_invariant incr. logical_simplify.
-        subst. cbn. ssplit.
-        - auto.
-        - intros. discriminate.
-        - intros. auto.
+        subst. cbn. ssplit; intros; [auto|discriminate|auto].
       }
-      eapply incr_invariant_preserved in Hinv as Hinv'; [|reflexivity].
-      unfold counter_related. exists (update_repr (c:=incr) (h2d, tt) repr).
-      rewrite surjective_pairing with (A:=counter_device) (B:=tl_d2h)
-                                      (p:=Semantics.step incr sL1 (h2d, tt)) in Hstep.
-      apply pair_equal_spec in Hstep. destruct Hstep as [Hstep1 Hstep2]. subst.
-      split; [| apply Hinv'; apply Hprec].
-      inversion Hrel; subst;
+      exists repr'; split; [|auto].
+      inversion_rel_spec; inversion_rel_base;
         destruct_tl_h2d; destruct_tl_d2h; tlsimpl; subst;
           cbn in sL1; destruct sL1 as ((?busy, (?done, (?regs, ?d2h))), (?s_tl, ?s_inner));
-            simplify_invariant incr; logical_simplify; subst;
-              cbn -[replace].
-      all: try (destruct x as [|[|[|]]]);
-        destruct (outstanding_h2d r_tl), d_ready;
-        try destruct (TLUL.a_opcode t =? Get)%N, (TLUL.a_opcode t =? PutFullData)%N;
-        try (rewrite incrN_word_to_bv);
-        boolsimpl; constructor; try assumption.
-      all: destruct H6; subst; destruct r_regs; cbn in H |- *; assumption.
-    - (* state_machine_read_to_device_read: *)
-      (* simpler because device.maxRespDelay=1 *)
-      intros ? ? ? ? [v [sH'' Hex_read]] [repr Hrel].
-      cbn in Hex_read. logical_simplify. rewrite  H1.
-      unfold counter_related.
-      match goal with
-      | |- context [ device.runUntilResp ?x _ _ ] =>
-        remember x as h2d eqn:Eh2d; replace x with h2d
-      end.
-      assert (Hprec: precondition incr (h2d, tt) repr).
-      { destruct_tl_h2d. tlsimpl.
-        cbn in sL; destruct sL as ((?busy, (?done, (?regs, ?d2h))), (?s_tl, ?s_inner)).
-        destruct repr as (((?r_state, ?r_regs), ?r_tl), ?r_inner).
-        simplify_invariant incr. logical_simplify.
-        subst. cbn. ssplit; intros; auto.
-      }
-      pose (r_ := r). destruct r.
-      + (* r=VALUE *)
-        pose (sH_ := sH); destruct sH; cbn in H2; try (exfalso; assumption); logical_simplify; subst.
-        inversion H; subst.
-        eapply runUntilResp_big_step with (s:=sL) in Hprec
-          as [n [inputs [sL' [repr' [d2h [sL'' [HrunU [HmaxRespDelay [Einputs [EsL' [Erepr' [Hpostc' [Ed_valid Hinv'']]]]]]]]]]]]]; subst; auto.
-        exists d2h, sL'', IDLE.
-        ssplit.
-        3: cbn; ssplit; try reflexivity; [].
-        * assumption.
-        * eexists.
-          split; [|apply Hinv''].
+            simplify_invariant incr; logical_simplify; subst; cbn -[replace];
+              apply No_inflight; try (constructor; lia); [].
+      replace ((word_to_N val + 1) mod 4294967296)%N with
+          (word_to_N (word.add (word.of_Z 1) val)) by
+          (unfold word_to_N; ZnWords);
+        apply BUSY_done_related.
+
+    - (* [state_machine_read_to_device_send_read_or_later] *)
+      intros ? ? ? ? ? ? [v [sH'' Hex_read]] [repr [Hrel Hinv]] **.
+      cbn in Hex_read. logical_simplify.
+      rewrite H5. clear H5.
+      use_spec.
+      1: simplify_spec incr; simplify_spec (tlul_adapter_reg (reg_count:=2)); simplify_spec Incr.inner;
+        simplify_invariant incr;
+        cbn in sL; destruct sL as ((?busy, (?done, (?regs, ?d2h))), (?s_tl, ?s_inner));
+          destruct repr as ((((?r_state, ?r_prev_state), ?r_regs), ?r_tl), ?r_inner);
+          destruct_tl_h2d; tlsimpl; logical_simplify; subst;
+            ssplit; intros; auto.
+
+      destruct_one_match; [destruct_one_match|].
+      (* case 1: device ready, valid response
+           In our TL implementation [a_ready = negb d_valid], hence this case
+           is not possible.
+           case 3: device not ready
+           If the inflight queue is empty, the device must be ready, hence
+           this case is not possible. *)
+      1,3: exfalso;
+        unfold device.last_d2h, counter_device in *;
+        cbn in sL; destruct sL as ((?busy, (?done, (?regs, ?d2h))), (?s_tl, ?s_inner));
+          destruct repr as ((((?r_state, ?r_prev_state), ?r_regs), ?r_tl), ?r_inner);
+          simplify_invariant incr; subst; logical_simplify; destruct_tl_d2h; tlsimpl; subst;
+          inversion_rel_spec; logical_simplify; discriminate.
+      (* device ready, no valid response: *)
+      ssplit.
+      1: eexists; split; [|eassumption]; [].
+      all:
+        unfold device.tl_inflight_ops, device.last_d2h, device.maxRespDelay,
+        counter_device, counter_related in *;
+        cbn in sL; destruct sL as ((?busy, (?done, (?regs, ?d2h))), (?s_tl, ?s_inner));
+          cbn in sL'; destruct sL' as ((?busy, (?done, (?regs, ?d2h))), (?s_tl, ?s_inner));
+            destruct repr as ((((?r_state, ?r_prev_state), ?r_regs), ?r_tl), ?r_inner);
+            destruct_tl_d2h; destruct_tl_h2d;
+              simplify_spec incr; simplify_spec (tlul_adapter_reg (reg_count:=2));
+                simplify_invariant incr;
+                logical_simplify; tlsimpl; subst;
+                  cbn in Hinv'; logical_simplify; subst.
+      + destruct r.
+        * (* [r:=VALUE] *)
+          inversion_rel_spec; inversion_rel_base; destruct H6; subst.
+          cbn; replace (N.land (word_to_N (word.of_Z 16384)) 4) with 0%N
+            by (rewrite Z_word_N by lia; reflexivity);
+          cbn; eapply Inflight_read_value; [eauto| |reflexivity..].
+          logical_simplify. assumption.
+        * (* [r:=STATUS] *)
+          inversion_rel_spec; inversion_rel_base; subst; logical_simplify; subst; cbn.
+            eapply Inflight_read_status; try (constructor; lia).
+          all: replace (N.land (word_to_N (word.of_Z 16388)) 4) with 4%N
+            by (rewrite Z_word_N by lia; reflexivity); eauto.
+          all: cbn; replace ((word_to_N val + 1) mod 4294967296)%N with
+                        (word_to_N (word.add (word.of_Z 1) val)) by
+              (unfold word_to_N; ZnWords); constructor.
+
+      + inversion_rel_spec; inversion_rel_base; subst; logical_simplify; subst; lia.
+
+    - (* [state_machine_read_to_device_ack_read_or_later] *)
+      intros ? ? ? ? ? ? [v [sH'' Hex_read]] [repr [Hrel Hinv]] **.
+      (* assert (Hex_rel: exists sL'' h2d', device.run1 sL'' (set_d_ready true h2d') = sL /\ *)
+      (*                               counter_related sH sL'' []). *)
+      (* { admit. } *)
+      (* logical_simplify. destruct H0 as [repr'' [Hrel'' Hinv'']]. *)
+      (* use_spec. 1: admit. *)
+      (* rename Hprec into Hprec''. rename repr' into repr'''. rename Erepr' into Erepr''. rename Hinv' into Hinv'''. *)
+      cbn in Hex_read. logical_simplify.
+      rewrite H2. clear H2. rename H3 into Hex_read.
+      use_spec.
+      1: simplify_spec incr; simplify_spec (tlul_adapter_reg (reg_count:=2)); simplify_spec Incr.inner;
+        simplify_invariant incr;
+        cbn in sL; destruct sL as ((?busy, (?done, (?regs, ?d2h))), (?s_tl, ?s_inner));
+          destruct repr as (((?r_state, ?r_regs), ?r_tl), ?r_inner);
+          destruct r_state;
+          destruct_tl_h2d; tlsimpl; logical_simplify; subst;
+            ssplit; intros; auto.
+
+      destruct_one_match.
+      (* case 2: no valid response
+         If the inflight queue is not empty, the device must be sending a
+         response, hence this case is not possible. *)
+      2: unfold device.last_d2h, counter_device in *;
+        cbn in sL; destruct sL as ((?busy, (?done, (?regs, ?d2h))), (?s_tl, ?s_inner));
+          destruct repr as (((?r_state, ?r_regs), ?r_tl), ?r_inner);
+          simplify_invariant incr; subst; logical_simplify; destruct_tl_d2h; tlsimpl; subst;
+            inversion_rel_spec; try inversion_rel_base; logical_simplify; subst;
+              try destruct r_tl; logical_simplify; subst;
+                discriminate.
+
+      (* case 1: valid response *)
+      destruct r.
+      + (* [r:=VALUE] *)
+        inversion_rel_spec;
+          try (exfalso; destruct_tl_h2d; tlsimpl; subst; unfold word_to_N in *; cbn in *; ZnWords).
+
+        destruct Hex_read; subst.
+        logical_simplify; subst.
+        exists IDLE. ssplit.
+        * eexists. split; [|eassumption].
+          cbn.
+          cbn in sL; destruct sL as ((?busy, (?done, (?regs, ?d2h))), (?s_tl, ?s_inner));
+            simplify_invariant incr;
+            logical_simplify; tlsimpl; subst.
+          apply No_inflight, IDLE_related.
+        * cbn. ssplit; try reflexivity.
+          clear Hinv'.
+          cbn in sL; destruct sL as ((?busy, (?done, (?regs, ?d2h))), (?s_tl, ?s_inner));
           simplify_invariant incr.
-          simplify_invariant Incr.inner.
-          simplify_invariant (tlul_adapter_reg (reg_count:=2)).
-          cbn in sL''; destruct sL'' as ((?busy, (?done, (?regs, ?d2h))), (?s_tl, ?s_inner)).
-          clear HrunU.
-          pose (n_:=n). destruct n as [|[|n]].
-          3: unfold device.maxRespDelay, counter_device in HmaxRespDelay; exfalso; lia.
-          all: cbn [repeat fold_left] in *.
-          -- destruct Hpostc' as [req' [h2d' [regs' [d2h' [io_re' [io_we' [io_address' [io_data' [io_mask' Hpostc']]]]]]]]].
-             logical_simplify.
-             cbn in H5.
-             destruct (outstanding_h2d r_tl) eqn:Houts.
-             ++ logical_simplify. rewrite Ed_valid in * |-. discriminate.
-             ++ cbn in H5. logical_simplify.
-                destruct_tl_d2h. tlsimpl. subst.
-                simplify_invariant incr.
-                cbn in sL; destruct sL as ((?busy, (?done, (?regs, ?d2h))), (?s_tl, ?s_inner)).
-                cbn in Hinv'' |- *.
-                rewrite Houts in Hinv'' |- *. cbn in Hinv''. logical_simplify.
-                cbn in *.
-                logical_simplify. subst.
-                rewrite Z_word_N in * by lia. cbn in *. logical_simplify. subst.
-                apply IDLE_related.
-          -- cbn in Hpostc'.
-             destruct (outstanding_h2d r_tl) eqn:Houts;
-             destruct Hpostc' as [req' [h2d' [regs' [d2h' [io_re' [io_we' [io_address' [io_data' [io_mask' Hpostc']]]]]]]]];
-             logical_simplify;
-             cbn in H5; rewrite Houts in H5; cbn in H5; logical_simplify; subst.
-             ++ destruct_tl_d2h. tlsimpl. subst.
-                simplify_invariant incr.
-                cbn in sL; destruct sL as ((?busy, (?done, (?regs, ?d2h))), (?s_tl, ?s_inner)).
-                cbn in Hinv'' |- *.
-                rewrite Houts in Hinv'' |- *. cbn in Hinv'' |- *. logical_simplify.
-                rewrite Houts. cbn.
-                rewrite Z_word_N in * by lia. cbn in *.
-                destruct H8; subst; apply IDLE_related.
-             ++ rewrite Ed_valid in * |-. discriminate.
-        * pose (n_:=n). destruct n as [|[|n]].
-          -- cbn [repeat fold_left] in *.
-             destruct Hpostc' as [req' [h2d' [regs' [d2h' [io_re' [io_we' [io_address' [io_data' [io_mask' Hpostc']]]]]]]]].
-             logical_simplify.
-             cbn in H5.
-             destruct (outstanding_h2d r_tl) eqn:Houts.
-             ++ logical_simplify. rewrite Ed_valid in * |-. discriminate.
-             ++ cbn in H5. logical_simplify.
-                destruct_tl_d2h. tlsimpl. subst.
-                simplify_invariant incr.
-                cbn in sL; destruct sL as ((?busy, (?done, (?regs, ?d2h))), (?s_tl, ?s_inner)).
-                cbn in sL''; destruct sL'' as ((?busy, (?done, (?regs, ?d2h))), (?s_tl, ?s_inner)).
-                cbn in Hinv''.
-                rewrite Houts in Hinv''. cbn in Hinv''. logical_simplify.
-                cbn in *.
-                logical_simplify. subst.
-                rewrite Z_word_N in * by lia. cbn in *. logical_simplify. subst.
-                rewrite H3. apply N_to_word_word_to_N.
-          -- cbn [repeat fold_left] in *.
-             cbn in Hpostc'.
-             destruct (outstanding_h2d r_tl) eqn:Houts;
-             destruct Hpostc' as [req' [h2d' [regs' [d2h' [io_re' [io_we' [io_address' [io_data' [io_mask' Hpostc']]]]]]]]];
-             logical_simplify;
-             cbn in H5; rewrite Houts in H5; cbn in H5; logical_simplify; subst.
-             ++ destruct_tl_d2h. tlsimpl. subst.
-                simplify_invariant incr.
-                cbn in sL; destruct sL as ((?busy, (?done, (?regs, ?d2h))), (?s_tl, ?s_inner)).
-                cbn in sL''; destruct sL'' as ((?busy, (?done, (?regs, ?d2h))), (?s_tl, ?s_inner)).
-                cbn in Hinv''.
-                rewrite Houts in Hinv''. cbn in Hinv''. logical_simplify.
-                rewrite Z_word_N in * by lia. cbn -[replace] in *.
-                destruct H8; subst; destruct r_regs; cbn in H3 |- *;
-                  rewrite H3; apply N_to_word_word_to_N.
-             ++ rewrite Ed_valid in * |-. discriminate.
-          -- unfold device.maxRespDelay, counter_device in HmaxRespDelay. exfalso. lia.
-      + (* r=STATUS *)
-        eapply runUntilResp_big_step in Hprec as [n [inputs [sL' [repr' [d2h [sL'' [HrunU [HmaxRespDelay [Einputs [EsL' [Erepr' [Hpostc' [Ed_valid Hinv'']]]]]]]]]]]]]; subst; auto; [|eassumption].
-        inversion H; subst.
-        * do 3 eexists; ssplit.
-          -- rewrite HrunU; reflexivity.
-          -- eexists; split; [|eassumption];
-               destruct n as [|[|n]];
-               [| |unfold device.maxRespDelay, counter_device in HmaxRespDelay; exfalso; lia];
-               cbn [repeat fold_left] in *;
-               simplify_invariant incr;
-               cbn in sL; destruct sL as ((?busy, (?done, (?regs, ?d2h))), (?s_tl, ?s_inner));
-                 logical_simplify; subst;
-                   cbn; destruct (outstanding_h2d r_tl) eqn:Eouts;
-                     try (cbn; rewrite Eouts; cbn);
-                     apply IDLE_related.
-          -- cbn. ssplit; try reflexivity.
-             destruct n as [|[|n]];
-               [| |unfold device.maxRespDelay, counter_device in HmaxRespDelay; exfalso; lia];
-               cbn [repeat fold_left] in *; simplify_spec incr;
-                 simplify_spec (tlul_adapter_reg (reg_count:=2)).
-             ++ destruct Hpostc' as [req' [h2d' [regs' [d2h' [io_re' [io_we' [io_address' [io_data' [io_mask' Hpostc']]]]]]]]]; logical_simplify; cbn in H5;
-                  destruct (outstanding_h2d r_tl) eqn:Eouts;
-                  [logical_simplify; rewrite Ed_valid in *; discriminate|];
-                  cbn in H5; logical_simplify; rewrite H9.
-                unfold status_value, STATUS_IDLE, N_to_word, word_to_N.
-                simplify_invariant incr.
-                cbn in sL; destruct sL as ((?busy, (?done, (?regs, ?d2h))), (?s_tl, ?s_inner)).
-                logical_simplify.
-                replace (N.to_nat ((N.land (Z.to_N (word.unsigned (word.of_Z 16388))) 4 / 4) mod 1073741824)) with 1.
-                ** ZnWords.
-                ** ZnWords_pre. rewrite Zmod_small; [|lia].
-                   rewrite N.mod_small; cbn; lia.
-             ++ admit.
-        * admit.
-        * admit.
-        * admit.
-    - (* state_machine_write_to_device_write: *)
-      admit.
+          logical_simplify; subst.
+          destruct_tl_h2d; tlsimpl; subst.
+          rewrite H19. cbn. rewrite H3. apply N_to_word_word_to_N.
+      + (* [r:=STATUS] *)
+        inversion_rel_spec;
+          try (exfalso; destruct_tl_h2d; tlsimpl; subst; unfold word_to_N in *; cbn in *; ZnWords).
+
+        inversion_rel_base;
+          cbn in sL |- *; destruct sL as ((?busy, (?done, (?regs, ?d2h))), (?s_tl, ?s_inner));
+            simplify_invariant incr;
+            logical_simplify; subst; logical_simplify; subst;
+              match goal with
+              | H: d_data _ = _ |- _ =>
+                rewrite H
+              end;
+              cbn; destruct_tl_h2d; tlsimpl; subst; cbn;
+              change (Pos.to_nat 1) with 1.
+                (* match goal with *)
+                (* | H: nth 1 r_tl_regs 0%N = _ |- _ => rewrite H *)
+                (* end; *)
+                (* unfold N_to_word, status_value. *)
+        * eexists; ssplit; try reflexivity.
+          -- eexists.
+             ssplit; [|eassumption].
+             apply No_inflight. constructor.
+          -- assert (Hprev: r_prev_state = RSIdle) by admit.
+             subst.
+             match goal with
+             | H: nth 1 r_tl_regs 0%N = _ |- _ => rewrite H
+             end; unfold N_to_word, status_value.
+             ZnWords.
+        * destruct ncycles as [|ncycles]; [lia|].
+          eexists; ssplit; try reflexivity.
+          -- eexists. ssplit; [|eassumption].
+             apply No_inflight, BUSY2_related. apply lt_S_n. eauto.
+          -- right. eexists. ssplit; [reflexivity| |reflexivity].
+             assert (Hprev: exists d, r_prev_state = RSBusy d) by admit.
+             logical_simplify; subst.
+             match goal with
+             | H: nth 1 r_tl_regs 0%N = _ |- _ => rewrite H
+             end; unfold N_to_word, status_value.
+             ZnWords.
+        * destruct ncycles as [|ncycles]; [lia|].
+          eexists. ssplit; try reflexivity.
+          -- eexists. ssplit; [|eassumption].
+             cbn; rewrite incrN_word_to_bv.
+             apply No_inflight, BUSY_done_related.
+          -- right. eexists. ssplit; [reflexivity| |reflexivity].
+             assert (Hprev: exists d, r_prev_state = RSBusy d) by admit.
+             logical_simplify; subst.
+             match goal with
+             | H: nth 1 r_tl_regs 0%N = _ |- _ => rewrite H
+             end; unfold N_to_word, status_value.
+             ZnWords.
+        * eexists; ssplit; try reflexivity.
+          -- eexists. ssplit; [|eassumption].
+             apply No_inflight, DONE_related.
+          -- left. ssplit; [|reflexivity].
+             assert (Hprev: exists d, r_prev_state = RSDone d) by admit.
+             logical_simplify; subst; logical_simplify;
+             match goal with
+             | H: nth 1 r_tl_regs 0%N = _ |- _ => rewrite H
+             end; unfold N_to_word, status_value.
+             ZnWords.
+        * eexists; ssplit; try reflexivity.
+          -- eexists. ssplit; [|eassumption].
+             apply No_inflight, DONE_related.
+          -- assert (Hprev: exists d, r_prev_state = RSDone d) by admit.
+             logical_simplify; subst; logical_simplify.
+             match goal with
+             | H: nth 1 r_tl_regs 0%N = _ |- _ => rewrite H
+             end; unfold N_to_word, status_value.
+             ZnWords.
+
+    - (* [state_machine_write_to_device_send_write_or_later] *)
+      intros ? ? ? ? ? ? ? [sH'' [Hpow2 Hex_write]] [repr [Hrel Hinv]] **.
+      rewrite Hpow2. clear Hpow2.
+      use_spec.
+      1: simplify_spec incr; simplify_spec (tlul_adapter_reg (reg_count:=2)); simplify_spec Incr.inner;
+        simplify_invariant incr;
+        cbn in sL; destruct sL as ((?busy, (?done, (?regs, ?d2h))), (?s_tl, ?s_inner));
+          destruct repr as ((((?r_state, ?r_prev_state), ?r_regs), ?r_tl), ?r_inner);
+          destruct_tl_h2d; tlsimpl; logical_simplify; subst;
+            ssplit; intros; auto.
+
+      destruct_one_match; [destruct_one_match|].
+        (* case 1: device ready, valid response
+           In our TL implementation [a_ready = negb d_valid], hence this case
+           is not possible.
+           case 3: device not ready
+           If the inflight queue is empty, the device must be ready, hence
+           this case is not possible. *)
+      1,3: exfalso;
+        unfold device.last_d2h, counter_device in *;
+        cbn in sL; destruct sL as ((?busy, (?done, (?regs, ?d2h))), (?s_tl, ?s_inner));
+        destruct repr as ((((?r_state, ?r_prev_state), ?r_regs), ?r_tl), ?r_inner);
+          simplify_invariant incr; subst; logical_simplify; destruct_tl_d2h; tlsimpl; subst;
+            inversion_rel_spec; logical_simplify; discriminate.
+      (* device ready, no valid response: *)
+      ssplit.
+      1: eexists; split; [|eassumption]; [].
+      all:
+        unfold device.tl_inflight_ops, device.last_d2h, device.maxRespDelay,
+        counter_device, counter_related in *;
+        cbn in sL; destruct sL as ((?busy, (?done, (?regs, ?d2h))), (?s_tl, ?s_inner));
+          cbn in sL'; destruct sL' as ((?busy, (?done, (?regs, ?d2h))), (?s_tl, ?s_inner));
+            destruct repr as ((((?r_state, ?r_prev_state), ?r_regs), ?r_tl), ?r_inner);
+            destruct_tl_d2h; destruct_tl_h2d;
+              simplify_spec incr; simplify_spec (tlul_adapter_reg (reg_count:=2));
+                simplify_invariant incr;
+                logical_simplify; tlsimpl; subst;
+                  cbn in Hinv'; logical_simplify; subst.
+      + destruct r.
+        * (* [r:=VALUE] *)
+          inversion_rel_spec; inversion_rel_base; logical_simplify; subst; try contradiction.
+          cbn. apply Inflight_write_value; eauto; [].
+          rewrite Z_word_N by lia. change (Z.to_N 16384) with 16384%N. reflexivity.
+        * (* [r:=STATUS] *)
+          inversion_rel_spec; inversion_rel_base;
+          destruct Hex_write.
+      + inversion_rel_spec; inversion_rel_base; subst; logical_simplify; subst; lia.
+
+    - (* [state_machine_write_to_device_ack_write_or_later] *)
+      intros ? ? ? ? ? ? ? [sH'' [Hpow2 Hex_write]] [repr [Hrel Hinv]] **.
+      rewrite Hpow2 in *. clear Hpow2.
+      use_spec.
+      1: simplify_spec incr; simplify_spec (tlul_adapter_reg (reg_count:=2)); simplify_spec Incr.inner;
+        simplify_invariant incr;
+        cbn in sL; destruct sL as ((?busy, (?done, (?regs, ?d2h))), (?s_tl, ?s_inner));
+          destruct repr as ((((?r_state, ?r_prev_state), ?r_regs), ?r_tl), ?r_inner);
+          destruct_tl_h2d; tlsimpl; logical_simplify; subst;
+            ssplit; intros; auto.
+
+      destruct_one_match.
+      (* case 2: no valid response
+         If the inflight queue is not empty, the device must be sending a
+         response, hence this case is not possible. *)
+      2: unfold device.last_d2h, counter_device in *;
+        cbn in sL; destruct sL as ((?busy, (?done, (?regs, ?d2h))), (?s_tl, ?s_inner));
+          destruct repr as ((((?r_state, ?r_prev_state), ?r_regs), ?r_tl), ?r_inner);
+          simplify_invariant incr; subst; logical_simplify; destruct_tl_d2h; tlsimpl; subst;
+            inversion_rel_spec; try inversion_rel_base; logical_simplify; subst;
+              try destruct r_tl; logical_simplify; subst;
+                discriminate.
+
+      (* case 1: valid response *)
+      destruct r.
+      + (* [r:=VALUE] *)
+        inversion_rel_spec;
+          try (exfalso; destruct_tl_h2d; tlsimpl; subst; unfold word_to_N in *; cbn in *; ZnWords).
+
+        destruct Hex_write; subst.
+        logical_simplify; subst.
+        eexists. ssplit; [|cbn; split; reflexivity].
+        eexists. split; [|eassumption].
+        cbn.
+        cbn in sL; destruct sL as ((?busy, (?done, (?regs, ?d2h))), (?s_tl, ?s_inner));
+            simplify_invariant incr;
+            logical_simplify; tlsimpl; subst.
+        apply No_inflight.
+        simplify_invariant Incr.inner; destruct s_inner; logical_simplify.
+        destruct x as [|[|[|]]]; [exfalso; lia|..| exfalso; lia];
+          destruct_tl_h2d; tlsimpl; subst;
+            match goal with
+            | H: word_to_N v = word_to_N val |- _ =>
+              rewrite <- H
+            end.
+        * constructor; lia.
+        * replace ((word_to_N v + 1) mod 4294967296)%N with
+                        (word_to_N (word.add (word.of_Z 1) v)) by
+              (unfold word_to_N; ZnWords).
+          constructor.
+      + (* [r:=STATUS] *)
+        inversion_rel_spec;
+          try (exfalso; destruct_tl_h2d; tlsimpl; subst; unfold word_to_N in *; cbn in *; ZnWords).
     - (* read_step_unique: *)
       intros. simpl in *. unfold read_step in *. simp.
       destruct v; destruct r; try contradiction; simp; try reflexivity.
